Finished BoundVars

src/Language/PlutusIR/Analysis/BoundVars.v
@@ -19,171 +19,198 @@ Import NamedTerm.
 
 From QuickChick Require Import QuickChick.
 
-Module Ty.
 
-  Inductive appears_bound_in (X: tyname) : Ty -> Prop :=
-    | ABI_TyFun1 : forall T1 T2,
-        appears_bound_in X T1 ->
-        appears_bound_in X (Ty_Fun T1 T2)
-    | ABI_TyFun2 : forall T1 T2,
-        appears_bound_in X T2 ->
-        appears_bound_in X (Ty_Fun T1 T2)
-    | ABI_TyIFix1 : forall F T,
-        appears_bound_in X F ->
-        appears_bound_in X (Ty_IFix F T)
-    | ABI_TyIFix2 : forall F T,
-        appears_bound_in X T ->
-        appears_bound_in X (Ty_IFix F T)
-    | ABI_TyForall1 : forall K T,
-        appears_bound_in X (Ty_Forall X K T)
-    | ABI_TyForall2 : forall Y K T,
-        X <> Y ->
-        appears_bound_in Y T ->
-        appears_bound_in X (Ty_Forall Y K T)
-    | ABI_TyLam1 : forall K T,
-        appears_bound_in X (Ty_Lam X K T)
-    | ABI_TyLam2 : forall Y K T,
-        X <> Y ->
-        appears_bound_in Y T ->
-        appears_bound_in X (Ty_Lam Y K T)
-    | ABI_TyApp1 : forall T1 T2,
-        appears_bound_in X T1 ->
-        appears_bound_in X (Ty_App T1 T2)
-    | ABI_TyApp2 : forall T1 T2,  
-        appears_bound_in X T2 ->
-        appears_bound_in X (Ty_App T1 T2).
+Inductive appears_bound_in_ty (X: tyname) : Ty -> Prop :=
+  | ABIT_TyFun1 : forall T1 T2,
+      appears_bound_in_ty X T1 ->
+      appears_bound_in_ty X (Ty_Fun T1 T2)
+  | ABIT_TyFun2 : forall T1 T2,
+      appears_bound_in_ty X T2 ->
+      appears_bound_in_ty X (Ty_Fun T1 T2)
+  | ABIT_TyIFix1 : forall F T,
+      appears_bound_in_ty X F ->
+      appears_bound_in_ty X (Ty_IFix F T)
+  | ABIT_TyIFix2 : forall F T,
+      appears_bound_in_ty X T ->
+      appears_bound_in_ty X (Ty_IFix F T)
+  | ABIT_TyForall1 : forall K T,
+      appears_bound_in_ty X (Ty_Forall X K T)
+  | ABIT_TyForall2 : forall Y K T,
+      X <> Y ->
+      appears_bound_in_ty Y T ->
+      appears_bound_in_ty X (Ty_Forall Y K T)
+  | ABIT_TyLam1 : forall K T,
+      appears_bound_in_ty X (Ty_Lam X K T)
+  | ABIT_TyLam2 : forall Y K T,
+      X <> Y ->
+      appears_bound_in_ty Y T ->
+      appears_bound_in_ty X (Ty_Lam Y K T)
+  | ABIT_TyApp1 : forall T1 T2,
+      appears_bound_in_ty X T1 ->
+      appears_bound_in_ty X (Ty_App T1 T2)
+  | ABIT_TyApp2 : forall T1 T2,  
+      appears_bound_in_ty X T2 ->
+      appears_bound_in_ty X (Ty_App T1 T2).
 
-  Derive DecOpt for (appears_bound_in x ty).
-  
-  Instance appears_bound_in_decopt_sound x ty: DecOptSoundPos (appears_bound_in x ty).
-  Proof. derive_sound. Qed.
+QCDerive DecOpt for (appears_bound_in_ty x ty).  
 
-End Ty.
+Instance appears_bound_in_tm_decopt_sound x ty: DecOptSoundPos (appears_bound_in_ty x ty).
+Proof. derive_sound. Qed.
 
-Module Term.
+(* TODO: works, but slows down compilation when using make
+   Instance appears_bound_in_tm_decopt_complte x ty: DecOptCompletePos (appears_bound_in_ty x ty).
+   Proof. derive_complete. Qed.
+ *)
 
-  Definition bv_constructor (c : constructor) : string :=
-    match c with
-    | Constructor (VarDecl x _) _ => x
-    end.
+Definition bv_constructor (c : constructor) : string :=
+  match c with
+  | Constructor (VarDecl x _) _ => x
+  end.
 
-  Definition map_bv_constructor := map bv_constructor.
+(* QuickChick will fail to derive a checker for appears_bound_in if this application
+ * occurs directly in the constructor. This is because QuickChick will try and match
+ * 'bv_constructor' with the variables bound by the 'forall', which will fail.
+ *
+ * In short, only the function is allowed to be defined outside the constructor, and
+ * any variables applied to the function should be bound as quantified variables.
+ *)
+Definition map_bv_constructor := map bv_constructor.
 
-  Inductive appears_bound_in (x : name) : Term -> Prop :=
-    | ABI_LamAbs1 : forall T t,
-        appears_bound_in x (LamAbs x T t)
-    | ABI_LamAbs2 : forall y T t,
-        x <> y ->
-        appears_bound_in x t ->
-        appears_bound_in x (LamAbs y T t)
-    | ABI_Apply1 : forall t1 t2,
-        appears_bound_in x t1 ->
-        appears_bound_in x (Apply t1 t2)
-    | ABI_Apply2 : forall t1 t2,
-        appears_bound_in x t2 ->
-        appears_bound_in x (Apply t1 t2)
-    | ABI_TyAbs : forall X K t,
-        appears_bound_in x t ->
-        appears_bound_in x (TyAbs X K t)
-    | ABI_TyInst : forall t T,
-        appears_bound_in x t ->
-        appears_bound_in x (TyInst t T)
-    | ABI_IWrap : forall F T t,
-        appears_bound_in x t ->
-        appears_bound_in x (IWrap F T t)
-    | ABI_Unwrap : forall t,
-        appears_bound_in x t ->
-        appears_bound_in x (Unwrap t)
-    | ABI_Let_Nil : forall recty t0,
-        appears_bound_in x t0 ->
-        appears_bound_in x (Let recty nil t0)
-    | ABI_Let_Cons : forall recty b bs t0,
-        appears_bound_in x (Let recty bs t0) ->
-        appears_bound_in x (Let recty (b :: bs) t0)
-    | ABI_Let_TermBind1 : forall recty stricty T t bs t0,
-        appears_bound_in x (Let recty (TermBind stricty (VarDecl x T) t :: bs) t0)
-    | ABI_Let_TermBind2 : forall recty stricty y T t bs t0,
-        appears_bound_in x t ->
-        appears_bound_in x (Let recty (TermBind stricty (VarDecl y T) t :: bs) t0)
-    | ABI_Let_DatatypeBind : forall recty XK YKs mfunc cs t0 bs,
-        In x (mfunc :: map_bv_constructor cs) ->
-        appears_bound_in x (Let recty (DatatypeBind (Datatype XK YKs mfunc cs) :: bs) t0) 
-    .
+Inductive appears_bound_in_tm (x : name) : Term -> Prop :=
+  | ABITM_LamAbs1 : forall T t,
+      appears_bound_in_tm x (LamAbs x T t)
+  | ABITM_LamAbs2 : forall y T t,
+      x <> y ->
+      appears_bound_in_tm x t ->
+      appears_bound_in_tm x (LamAbs y T t)
+  | ABITM_Apply1 : forall t1 t2,
+      appears_bound_in_tm x t1 ->
+      appears_bound_in_tm x (Apply t1 t2)
+  | ABITM_Apply2 : forall t1 t2,
+      appears_bound_in_tm x t2 ->
+      appears_bound_in_tm x (Apply t1 t2)
+  | ABITM_TyAbs : forall X K t,
+      appears_bound_in_tm x t ->
+      appears_bound_in_tm x (TyAbs X K t)
+  | ABITM_TyInst : forall t T,
+      appears_bound_in_tm x t ->
+      appears_bound_in_tm x (TyInst t T)
+  | ABITM_IWrap : forall F T t,
+      appears_bound_in_tm x t ->
+      appears_bound_in_tm x (IWrap F T t)
+  | ABITM_Unwrap : forall t,
+      appears_bound_in_tm x t ->
+      appears_bound_in_tm x (Unwrap t)
+  | ABITM_Let_Nil : forall recty t0,
+      appears_bound_in_tm x t0 ->
+      appears_bound_in_tm x (Let recty nil t0)
+  | ABITM_Let_Cons : forall recty b bs t0,
+      appears_bound_in_tm x (Let recty bs t0) ->
+        appears_bound_in_tm x (Let recty (b :: bs) t0)
+  | ABITM_Let_TermBind1 : forall recty stricty T t bs t0,
+      appears_bound_in_tm x (Let recty (TermBind stricty (VarDecl x T) t :: bs) t0)
+  | ABITM_Let_TermBind2 : forall recty stricty y T t bs t0,
+      appears_bound_in_tm x t ->
+      appears_bound_in_tm x (Let recty (TermBind stricty (VarDecl y T) t :: bs) t0)
+  | ABITM_Let_DatatypeBind : forall recty XK YKs mfunc cs t0 bs,
+      In x (mfunc :: map_bv_constructor cs) ->
+      appears_bound_in_tm x (Let recty (DatatypeBind (Datatype XK YKs mfunc cs) :: bs) t0) 
+      .
 
-  Derive DecOpt for (appears_bound_in x tm).
+(* Necessary since 'In' has strings as arguments *)
+(* TODO: move these elsewhere? In favour of deriving these once in a central place?*)
+QCDerive EnumSized for ascii.
+QCDerive EnumSized for string.
 
-End Term.
+QCDerive DecOpt for (appears_bound_in_tm x tm).
+
+(* TODO: finishes, but does not finalize a proof :(
+   Instance appears_bound_in_tm_decopt_sound x tm: DecOptSoundPos (appears_bound_in_tm x tm).
+   Proof. derive_sound. Qed.
+*)
+
+(* TODO: Does not terminate
+   Instance appears_bound_in_tm_decopt_complete x tm: DecOptCompletePos (appears_bound_in_tm x tm).
+   Proof. derive_complete. Qed.
+ *)
 
 
-Module Annotation.
+Inductive appears_bound_in_ann (X : tyname) : Term -> Prop :=
+  | ABIA_LamAbs1 : forall x T t,
+      appears_bound_in_ty X T ->
+      appears_bound_in_ann X (LamAbs x T t)
+  | ABIA_LamAbs : forall x T t,
+      appears_bound_in_ann X t ->
+      appears_bound_in_ann X (LamAbs x T t)
+  | ABIA_Apply1 : forall t1 t2,
+      appears_bound_in_ann X t1 ->
+      appears_bound_in_ann X (Apply t1 t2)
+  | ABIA_Apply2 : forall t1 t2,
+      appears_bound_in_ann X t2 ->
+      appears_bound_in_ann X (Apply t1 t2)
+  | ABIA_TyAbs1 : forall K t,
+      appears_bound_in_ann X (TyAbs X K t)
+  | ABIA_TyAbs2 : forall Y K t,
+      X <> Y ->
+      appears_bound_in_ann X t ->
+      appears_bound_in_ann X (TyAbs Y K t)
+  | ABIA_TyInst1 : forall t T,
+      appears_bound_in_ann X t ->
+      appears_bound_in_ann X (TyInst t T)
+  | ABIA_TyInst2 : forall t T,
+      appears_bound_in_ty X T ->
+      appears_bound_in_ann X (TyInst t T)
+  | ABIA_IWrap1 : forall F T t,
+      appears_bound_in_ty X F ->
+      appears_bound_in_ann X (IWrap F T t)
+  | ABIA_IWrap2 : forall F T t,
+      appears_bound_in_ty X T ->
+      appears_bound_in_ann X (IWrap F T t)
+  | ABIA_IWrap3 : forall F T t,
+      appears_bound_in_ann X t ->
+      appears_bound_in_ann X (IWrap F T t)
+  | ABIA_Unwrap : forall t,
+      appears_bound_in_ann X t ->
+      appears_bound_in_ann X (Unwrap t)
+  | ABIA_Error : forall T,
+      appears_bound_in_ty X T ->
+      appears_bound_in_ann X (Error T)
+  | ABIA_Let_Nil : forall recty t0,
+      appears_bound_in_ann X t0 ->
+      appears_bound_in_ann X (Let recty nil t0)
+  | ABIA_Let_Cons : forall recty b bs t0,
+      appears_bound_in_ann X (Let recty bs t0) ->
+        appears_bound_in_ann X (Let recty (b :: bs) t0)
+  | ABIA_Let_TermBind1 : forall recty stricty x T t bs t0,
+      appears_bound_in_ty X T ->
+      appears_bound_in_ann X (Let recty (TermBind stricty (VarDecl x T) t :: bs) t0)
+  | ABIA_Let_TermBind2 : forall recty stricty y T t bs t0,
+      appears_bound_in_ann X t ->
+      appears_bound_in_ann X (Let recty (TermBind stricty (VarDecl y T) t :: bs) t0)
+  | ABIA_Let_TypeBind1 : forall recty K T bs t0,
+      appears_bound_in_ann X (Let recty (TypeBind (TyVarDecl X K) T :: bs) t0)
+  | ABIA_Let_TypeBind2 : forall recty Y K T bs t0,
+      appears_bound_in_ty X T ->
+      appears_bound_in_ann X (Let recty (TypeBind (TyVarDecl Y K) T :: bs) t0)
+  | ABIA_Let_DatatypeBind : forall recty K YKs mfunc cs t0 bs,
+      appears_bound_in_ann X (Let recty (DatatypeBind (Datatype (TyVarDecl X K) YKs mfunc cs) :: bs) t0) 
+      .
 
-  Inductive appears_bound_in (X : tyname) : Term -> Prop :=
-    | ABI_LamAbs1 : forall x T t,
-        Ty.appears_bound_in X T ->
-        appears_bound_in X (LamAbs x T t)
-    | ABI_LamAbs : forall x T t,
-        appears_bound_in X t ->
-        appears_bound_in X (LamAbs x T t)
-    | ABI_Apply1 : forall t1 t2,
-        appears_bound_in X t1 ->
-        appears_bound_in X (Apply t1 t2)
-    | ABI_Apply2 : forall t1 t2,
-        appears_bound_in X t2 ->
-        appears_bound_in X (Apply t1 t2)
-    | ABI_TyAbs1 : forall K t,
-        appears_bound_in X (TyAbs X K t)
-    | ABI_TyAbs2 : forall Y K t,
-        X <> Y ->
-        appears_bound_in X t ->
-        appears_bound_in X (TyAbs Y K t)
-    | ABI_TyInst1 : forall t T,
-        appears_bound_in X t ->
-        appears_bound_in X (TyInst t T)
-    | ABI_TyInst2 : forall t T,
-        Ty.appears_bound_in X T ->
-        appears_bound_in X (TyInst t T)
-    | ABI_IWrap1 : forall F T t,
-        Ty.appears_bound_in X F ->
-        appears_bound_in X (IWrap F T t)
-    | ABI_IWrap2 : forall F T t,
-        Ty.appears_bound_in X T ->
-        appears_bound_in X (IWrap F T t)
-    | ABI_IWrap3 : forall F T t,
-        appears_bound_in X t ->
-        appears_bound_in X (IWrap F T t)
-    | ABI_Unwrap : forall t,
-        appears_bound_in X t ->
-        appears_bound_in X (Unwrap t)
-    | ABI_Error : forall T,
-        Ty.appears_bound_in X T ->
-        appears_bound_in X (Error T)
-    | ABI_Let_Nil : forall recty t0,
-        appears_bound_in X t0 ->
-        appears_bound_in X (Let recty nil t0)
-    | ABI_Let_Cons : forall recty b bs t0,
-        appears_bound_in X (Let recty bs t0) ->
-        appears_bound_in X (Let recty (b :: bs) t0)
-    | ABI_Let_TermBind1 : forall recty stricty x T t bs t0,
-        Ty.appears_bound_in X T ->
-        appears_bound_in X (Let recty (TermBind stricty (VarDecl x T) t :: bs) t0)
-    | ABI_Let_TermBind2 : forall recty stricty y T t bs t0,
-        appears_bound_in X t ->
-        appears_bound_in X (Let recty (TermBind stricty (VarDecl y T) t :: bs) t0)
-    | ABI_Let_TypeBind1 : forall recty K T bs t0,
-        appears_bound_in X (Let recty (TypeBind (TyVarDecl X K) T :: bs) t0)
-    | ABI_Let_TypeBind2 : forall recty Y K T bs t0,
-        Ty.appears_bound_in X T ->
-        appears_bound_in X (Let recty (TypeBind (TyVarDecl Y K) T :: bs) t0)
-    | ABI_Let_DatatypeBind : forall recty K YKs mfunc cs t0 bs,
-        appears_bound_in X (Let recty (DatatypeBind (Datatype (TyVarDecl X K) YKs mfunc cs) :: bs) t0) 
-    .
+QCDerive DecOpt for (appears_bound_in_ann x tm).
 
-End Annotation.
+Instance appears_bound_in_ann_decopt_sound x tm: DecOptSoundPos (appears_bound_in_ann x tm).
+Proof. derive_sound. Qed.
+
+(* TODO: Does not terminate
+Instance appears_bound_in_ann_decopt_complete x tm: DecOptCompletePos (appears_bound_in_ann x tm).
+Proof. derive_complete. Qed.
+*)
+
 
 #[export] Hint Constructors 
-  Ty.appears_bound_in 
-  Term.appears_bound_in
-  Annotation.appears_bound_in
+  appears_bound_in_ty
+  appears_bound_in_tm
+  appears_bound_in_ann
   : core.
 
 
@@ -233,7 +260,7 @@ Definition btvbs (bs : list binding') : list tyvar := List.concat (map btvb bs).
 
 Fixpoint bound_vars (t : term') : list var :=
  match t with
-   | Let rec bs t => concat (map bound_vars_binding bs) ++ bound_vars t
+   | Let rec bs t => List.concat (map bound_vars_binding bs) ++ bound_vars t
    | (LamAbs n ty t)   => n :: (bound_vars t)
    | (Var n)           => []
    | (TyAbs n k t)     => bound_vars t
@@ -251,17 +278,15 @@ with bound_vars_binding (b : binding') : list var := match b with
   | _                          => []
   end.
 
-Definition bound_vars_bindings := @concat _ ∘ map bound_vars_binding.
+Definition bound_vars_bindings := @List.concat _ ∘ map bound_vars_binding.
 
 End BoundVars.
 
-Import BoundVars.Term.
-
-Definition P_Term (t : Term) : Prop := Forall (fun v => appears_bound_in v t) (bound_vars t).
-Definition P_Binding (b : Binding) := Forall (fun v => forall t bs recty, appears_bound_in v (Let recty (b :: bs) t)) (bound_vars_binding b).
+Definition P_Term (t : Term) : Prop := Forall (fun v => appears_bound_in_tm v t) (bound_vars t).
+Definition P_Binding (b : Binding) := Forall (fun v => forall t bs recty, appears_bound_in_tm v (Let recty (b :: bs) t)) (bound_vars_binding b).
 
 Lemma bound_vars_appears_bound_in : (forall t, P_Term t) /\ (forall b, P_Binding b).
-Proof with eauto using appears_bound_in.
+Proof with eauto using appears_bound_in_tm.
   apply Term__multind with (P := P_Term) (Q := P_Binding).
   all: unfold P_Term...
   - intros.
@@ -284,12 +309,12 @@ Proof with eauto using appears_bound_in.
              apply ForallP_Forall in H.
              apply IHbs in H.
              eapply Forall_impl.
-             intros b. apply ABI_Let_Cons.
+             intros b. apply ABITM_Let_Cons.
              auto.
 
     + unfold P_Term in *.
-      eapply Forall_impl with (P := fun v => appears_bound_in v t)...
-      eauto using appears_bound_in.
+      eapply Forall_impl with (P := fun v => appears_bound_in_tm v t)...
+      eauto using appears_bound_in_tm.
       intros.
       induction bs...
       apply ForallP_Forall in H.
@@ -303,11 +328,11 @@ Proof with eauto using appears_bound_in.
     eauto.
   - intros.
     eapply Forall_cons...
-    eapply Forall_impl with (P := fun a => appears_bound_in a t0)...
+    eapply Forall_impl with (P := fun a => appears_bound_in_tm a t0)...
     intros. 
       destruct (string_dec a s).
-      * subst. apply ABI_LamAbs1.
-      * apply ABI_LamAbs2...
+      * subst. apply ABITM_LamAbs1.
+      * apply ABITM_LamAbs2...
 
   (* Common pattern: only need to prove an implication using a ABI rule *)
   Ltac tac rule :=
@@ -315,14 +340,14 @@ Proof with eauto using appears_bound_in.
 
   - intros.
     apply Forall_app. split.
-      + tac ABI_Apply1.
-      + tac ABI_Apply2.
+      + tac ABITM_Apply1.
+      + tac ABITM_Apply2.
   - intros. cbv. auto.
   - intros. cbv. auto.
-  - tac ABI_TyInst.
+  - tac ABITM_TyInst.
   - intros. cbv. auto.
-  - tac ABI_IWrap.
-  - tac ABI_Unwrap.
+  - tac ABITM_IWrap.
+  - tac ABITM_Unwrap.
   - intros.
     unfold P_Binding.
     intros.
@@ -330,8 +355,8 @@ Proof with eauto using appears_bound_in.
     destruct v.
     eapply Forall_cons.
       + intros...
-      + intros. eapply Forall_impl with (P := fun v => appears_bound_in v t).
-        1: { intros. apply ABI_Let_TermBind2... }
+      + intros. eapply Forall_impl with (P := fun v => appears_bound_in_tm v t).
+        1: { intros. apply ABITM_Let_TermBind2... }
         auto.
   - unfold P_Binding.
     intros.
@@ -341,11 +366,12 @@ Proof with eauto using appears_bound_in.
     destruct dtd.
     apply Forall_cons.
     + intros.
-      apply ABI_Let_DatatypeBind.
+      apply ABITM_Let_DatatypeBind.
       constructor...
     + apply Forall_forall.
       intros.
-      apply ABI_Let_DatatypeBind.
+      apply ABITM_Let_DatatypeBind.
+      apply In_Coq_In_equal.
       apply in_cons.
       assumption.
 Qed.
