Makefile
@@ -11,7 +11,7 @@ clean: Makefile.coq
 	rm -f Makefile.coq
 
 Makefile.coq: _CoqProject Makefile
-	coq_makefile COQFLAGS = "-w \"-all\"" -f _CoqProject | sed 's/$$(COQCHK) $$(COQCHKFLAGS) $$(COQLIBS)/$$(COQCHK) $$(COQCHKFLAGS) $$(subst -Q,-R,$$(COQLIBS))/' > Makefile.coq
+	coq_makefile COQFLAGS = "-w \"-all\"" -f _CoqProject -o Makefile.coq | sed 's/$$(COQCHK) $$(COQCHKFLAGS) $$(COQLIBS)/$$(COQCHK) $$(COQCHKFLAGS) $$(subst -Q,-R,$$(COQLIBS))/' > Makefile.coq
 
 _CoqProject: ;
 
